theories/types/utp_fset.thy
@@ -13,6 +13,7 @@ imports
   "../core/utp_event"
   "../tactics/utp_pred_tac"
   "../tactics/utp_expr_tac"
+  utp_list
 begin
 
 typedef 'a::DEFINED UFSET = "{xs :: 'a fset. \<forall>x\<in>\<^sub>fxs. \<D> x}"
@@ -20,14 +21,79 @@ typedef 'a::DEFINED UFSET = "{xs :: 'a fset. \<forall>x\<in>\<^sub>fxs. \<D> x}"
   apply (auto)
 done
 
-instantiation UFSET :: (DEFINED) DEFINED
+theorems Rep_UFSET' = Rep_UFSET [simplified]
+declare Rep_UFSET' [simp]
+declare Rep_UFSET_inverse [simp]
+theorems Abs_UFSET_inverse' = Abs_UFSET_inverse [simplified]
+declare Abs_UFSET_inverse' [simp]
+
+lemma Rep_UFSET_intro [intro!]:
+  "Rep_UFSET x = Rep_UFSET y \<Longrightarrow> x = y"
+  by (simp add:Rep_UFSET_inject)
+
+lemma Rep_UFSET_elim [elim]:
+  "\<lbrakk> x = y; Rep_UFSET x = Rep_UFSET y \<Longrightarrow> P \<rbrakk> \<Longrightarrow> P"
+  by (auto)
+
+setup_lifting type_definition_UFSET
+
+instantiation UFSET :: (DEFINED) DEFINED_NE
 begin
 definition "Defined_UFSET (xs :: 'a UFSET) = True"
-instance ..
+instance 
+  by (intro_classes, auto simp add:Defined_UFSET_def)
 end
 
 lemma Defined_UFSET [defined]: 
   "\<D> (xs :: ('a::DEFINED UFSET))"
   by (simp add:Defined_UFSET_def)
+
+lift_definition EmptyUF :: "'a::DEFINED UFSET" is "fempty"
+  by simp
+
+definition InsertUF :: "'a::DEFINED \<Rightarrow> 'a UFSET \<Rightarrow> 'a UFSET" where
+"InsertUF x xs = Abs_UFSET (finsert x (Rep_UFSET xs))"
+
+lemma InsertUF_rep_eq: 
+  "\<D> x \<Longrightarrow> Rep_UFSET (InsertUF x xs) = finsert x (Rep_UFSET xs)"
+  apply (subgoal_tac "(\<forall>y\<in>\<^sub>f(finsert x (Rep_UFSET xs)). \<D> y)")
+  apply (auto simp add:InsertUF_def)
+done
+
+lift_definition MemberUF :: "'a::DEFINED \<Rightarrow> 'a UFSET \<Rightarrow> bool" is "fmember"
+  by (auto)
+
+lift_definition NMemberUF :: "'a::DEFINED \<Rightarrow> 'a UFSET \<Rightarrow> bool" is "fnmember"
+  by (auto)
+
+lift_definition UnionUF :: "'a::DEFINED UFSET \<Rightarrow> 'a UFSET \<Rightarrow> 'a UFSET" is "funion"
+  by (auto)
+
+lift_definition InterUF :: "'a::DEFINED UFSET \<Rightarrow> 'a UFSET \<Rightarrow> 'a UFSET" is "finter"
+  by (auto)
+
+definition IntersyncUF :: 
+  "'a::DEFINED UFSET \<Rightarrow> 'a ULIST \<Rightarrow> 'a ULIST \<Rightarrow> ('a ULIST) UFSET"  where
+"IntersyncUF xs ys zs = Abs_UFSET (Abs_ULIST `\<^sub>f (intersync (Rep_UFSET xs) (Rep_ULIST ys) (Rep_ULIST zs)))"
+
+lemma UFSET_elems_defined [defined]:
+  "x \<in>\<^sub>f (Rep_UFSET xs) \<Longrightarrow> \<D> x"
+  apply (insert Rep_UFSET[of xs])
+  apply (auto)
+done
+
+text {* Set up the predicate and expression tactics to evaluate lists *}
+
+lemma UFSET_transfer [eval, evale]: 
+  "xs = ys \<longleftrightarrow> Rep_UFSET xs = Rep_UFSET ys"
+  by (auto)
+
+declare EmptyUF.rep_eq [eval, evale]
+declare InsertUF_rep_eq [eval, evale]
+declare UnionUF.rep_eq [eval, evale]
+declare InterUF.rep_eq [eval, evale]
+declare MemberUF.rep_eq [eval, evale]
+declare NMemberUF.rep_eq [eval, evale]
+declare IntersyncUF_def [eval, evale]
 
 end
