theories/parser/utp_pred_parser.thy
@@ -187,6 +187,7 @@ syntax
   "_pexpr_fset_inter"   :: "pexpr \<Rightarrow> pexpr \<Rightarrow> pexpr" (infixl "\<inter>" 70)
   "_pexpr_fset_member"  :: "pexpr \<Rightarrow> pexpr \<Rightarrow> pexpr" ("(_/ \<in> _)" [51, 51] 50)
   "_pexpr_fset_nmember" :: "pexpr \<Rightarrow> pexpr \<Rightarrow> pexpr" ("(_/ \<notin> _)" [51, 51] 50)
+  "_pexpr_intersync"    :: "pexpr \<Rightarrow> pexpr \<Rightarrow> pexpr \<Rightarrow> pexpr" (infixr "\<parallel>\<^bsub>_\<^esub>" 75)
   "_pexpr_event"        :: "NAME \<Rightarrow> pexpr \<Rightarrow> pexpr" ("_?_" 50)
 
 translations
@@ -235,6 +236,7 @@ translations
   "_pexpr_fset_inter xs ys"    == "CONST FInterPE xs ys"
   "_pexpr_fset_member x xs"    == "CONST FMemberPE x xs"
   "_pexpr_fset_nmember x xs"   == "CONST FNotMemberPE x xs"
+  "_pexpr_intersync p xs q"    == "CONST IntersyncPE xs p q"
   "_pexpr_event n v"           == "CONST EventPE n v"
 
 (* Linking the predicate parser to the poly parser *)
@@ -254,7 +256,7 @@ translations
 term "`($x)\<acute> = $y\<acute>`"
 term "`p[($x)\<acute>/y\<acute>]`"
 term "`\<lparr>true\<rparr>`"
- 
+
 lemma "`$x \<in> {<1>,<2>,<3>,<4>,<5>} \<sqsubseteq> $x = <1>`"
   by (utp_pred_tac)
 
